templates/multicopy/KT_flows.v
@@ -25,8 +25,1115 @@ Definition out_KT I k := ∃ t n, (k, t) ∈ outset_KT I n.
 
 Global Canonical Structure KT_flowint_ur : ucmraT := flowintUR KT_multiset.
 
+Definition gmap_decrement (kt: KT) (m : gmap KT nat) : gmap KT nat := 
+          if (1 <? m !!! kt) then <[kt := m !!! kt - 1]> m
+          else delete kt m.
+
+Lemma nzmap_decrement_wf (kt: KT) (m : gmap KT nat) :
+      nzmap_wf m → nzmap_wf (gmap_decrement kt m).
+Proof.
+  unfold nzmap_wf, map_Forall. intros Hm.
+  intros i x. destruct (decide (i = kt)).
+  - replace i. unfold gmap_decrement.
+    destruct (1 <? m !!! kt) eqn: Hmkt.
+    + rewrite lookup_insert. intros H'; inversion H'.
+      apply Nat.ltb_lt in Hmkt. 
+      unfold ccmunit, ccm_unit. simpl.
+      unfold nat_unit. lia.
+    + rewrite lookup_delete.
+      intros H'; inversion H'.
+  - unfold gmap_decrement. destruct (1 <? m !!! kt);
+    [ rewrite lookup_insert_ne; try done | rewrite lookup_delete_ne];
+    by pose proof Hm i x.       
+Qed.
+
+Definition nzmap_decrement (kt: KT) (m : nzmap KT nat) :=
+      let (m, Hm) := m in
+        NZMap (gmap_decrement kt m) (bool_decide_pack _ (nzmap_decrement_wf kt m 
+    (bool_decide_unpack _ Hm))).
+    
+Lemma nzmap_lookup_total_decrement kt m :
+      nzmap_decrement kt m ! kt = m ! kt - 1.
+Proof.
+  unfold nzmap_decrement. unfold nzmap_total_lookup.
+  destruct m as [mg prf_mg]. 
+  unfold lookup, nzmap_lookup.
+  unfold gmap_decrement.
+  destruct (1 <? mg !!! kt) eqn : Hari.
+  - apply Nat.ltb_lt in Hari.
+    rewrite lookup_insert. simpl.
+    unfold ccmunit, nat_unit.
+    destruct (mg !! kt) eqn: Hmg.
+    simpl. rewrite /(mg !!! kt).
+    unfold finmap_lookup_total.
+    rewrite Hmg. by simpl.
+    rewrite /(mg !!! kt).
+    unfold finmap_lookup_total.
+    rewrite Hmg. by simpl.
+  - apply Nat.ltb_ge in Hari.
+    rewrite lookup_delete. simpl.    
+    destruct (mg !! kt) eqn: Hmg.
+    simpl. rewrite /(mg !!! kt) in Hari.
+    unfold finmap_lookup_total in Hari.
+    rewrite Hmg in Hari. simpl in Hari.
+    unfold ccmunit, nat_unit. lia.
+    simpl. by unfold ccmunit, nat_unit.
+Qed.
+
+Lemma nzmap_lookup_total_decrement_ne kt m kt' :
+      kt' ≠ kt → nzmap_decrement kt m ! kt' = m ! kt'.
+Proof.
+  intros Hkt.
+  unfold nzmap_decrement. unfold nzmap_total_lookup.
+  destruct m as [mg prf_mg]. 
+  unfold lookup, nzmap_lookup.
+  unfold gmap_decrement.
+  destruct (1 <? mg !!! kt) eqn : Hari.
+  - rewrite lookup_insert_ne; try done.
+  - rewrite lookup_delete_ne; try done.
+Qed.
+
+
+Definition outflow_insert_KT (I : KT_flowint_ur) (n: Node) 
+                            (k: K) (t: nat) : KT_flowint_ur := 
+           let I_out_n := (<<[(k,t) := (out I n) ! (k,t) + 1 ]>> (out I n)) in
+           let I'_out := (<<[n := I_out_n]>> (out_map I)) in
+           (int {| infR := inf_map I ; outR := I'_out |}).
+
+Definition outflow_delete_KT (I : KT_flowint_ur) (n: Node) 
+                            (k: K) (t: nat) :KT_flowint_ur := 
+           let I_out_n := (nzmap_decrement (k,t) (out I n)) in
+           let I'_out := (<<[n := I_out_n]>> (out_map I)) in
+           (int {| infR := inf_map I ; outR := I'_out |}).
+
+Lemma outflow_insert_outset_ne_KT I n k t I' n' :
+      n' ≠ n → I' = outflow_insert_KT I n k t
+             → outset_KT I' n' = outset_KT I n'.
+Proof.
+  intros Hneq HeqI. unfold outset_KT.
+  unfold KT_flows.dom_ms.
+  replace I'. unfold outflow_insert_KT.
+  unfold out. simpl.
+  rewrite nzmap_lookup_total_insert_ne; try done.
+Qed.  
+
+Lemma outflow_insert_outset_KT I n k t I' :
+      I' = outflow_insert_KT I n k t → 
+           outset_KT I' n = (outset_KT I n) ∪ {[(k,t)]}.
+Proof.
+  intros Heq. unfold outset_KT.
+  unfold KT_flows.dom_ms.
+  replace I'. unfold outflow_insert_KT.
+  unfold out. simpl.
+  rewrite nzmap_lookup_total_insert.
+  apply leibniz_equiv.
+  rewrite nzmap_dom_insert_nonzero.
+  - set_solver.
+  - unfold ccmunit, ccm_unit. simpl.
+    unfold nat_unit. lia.
+Qed.
+
+Lemma outflow_delete_outset_ne_KT I n k t I' n' :
+      n' ≠ n → I' = outflow_delete_KT I n k t
+             → outset_KT I' n' = outset_KT I n'.
+Proof.
+  intros Hneq HeqI. unfold outset_KT.
+  unfold KT_flows.dom_ms.
+  replace I'. unfold out. simpl.
+  rewrite nzmap_lookup_total_insert_ne; try done.
+Qed.  
+
+Lemma outflow_delete_outset_KT I n k t I' :
+      I' = outflow_delete_KT I n k t → 
+         ((out I n ! (k,t) ≤ 1 → outset_KT I' n = (outset_KT I n) ∖ {[(k,t)]})
+          ∧ (1 < out I n ! (k,t) → outset_KT I' n = outset_KT I n)).
+Proof.
+  intros Heq. unfold outset_KT.
+  unfold KT_flows.dom_ms.
+  replace I'. unfold outflow_delete_KT.
+  unfold out. simpl. 
+  rewrite nzmap_lookup_total_insert.
+  unfold nzmap_decrement.
+  destruct (out_map I ! n) as [og prf_og] eqn:Ho.
+  unfold dom, nzmap_dom. simpl.
+  unfold gmap_decrement.
+  split.
+  - intros le_1.
+    unfold nzmap_total_lookup, lookup, nzmap_lookup in le_1.
+    destruct (1 <? og !!! (k, t)) eqn: Hog.
+    + apply Nat.ltb_lt in Hog.
+      rewrite /(og !!! (k, t)) in Hog.
+      unfold finmap_lookup_total in Hog.
+      unfold inhabitant in Hog.
+      simpl in Hog.
+      unfold ccmunit, ccm_unit in le_1. 
+      simpl in le_1. unfold nat_unit in le_1.
+      assert (∀ (x: nat), x ≤ 1 → x > 1 → False) as H'. lia. 
+      exfalso. apply (H' (default 0 (og !! (k,t)))); try done.
+    + rewrite Hog. apply Nat.ltb_ge in Hog.      
+      apply leibniz_equiv. by rewrite dom_delete.
+  - intros ge_1.
+    unfold nzmap_total_lookup, lookup, nzmap_lookup in ge_1.
+    assert (1 <? og !!! (k,t) = true) as H'.
+    { apply PeanoNat.Nat.ltb_lt. 
+      rewrite /(og !!! (k, t)).
+      unfold finmap_lookup_total.
+      unfold inhabitant. simpl.
+      unfold ccmunit, ccm_unit in ge_1; simpl in ge_1.
+      by unfold nat_unit in ge_1. }
+    rewrite H'. apply leibniz_equiv.
+    rewrite dom_insert.
+    assert ((k,t) ∈ dom (gset KT) og).
+    { rewrite elem_of_dom. destruct (og !! (k,t)) eqn: Hogkt.
+      unfold is_Some; exists n0; try done. rewrite Hogkt in ge_1.
+      unfold ccmunit, ccm_unit in ge_1; simpl in ge_1.
+      unfold nat_unit in ge_1; lia. }
+    set_solver.
+Qed.      
+
+(* assumes: n ∈ domm I *) 
+Definition inflow_insert_KT (I : KT_flowint_ur) (n: Node) 
+                            (k: K) (t: nat) :KT_flowint_ur := 
+           let I_inf_n := (<<[(k,t) := (inf I n) ! (k,t) + 1 ]>> (inf I n)) in
+           let I'_inf := (<[ n := I_inf_n ]>(inf_map I)) in
+           (int {| infR := I'_inf ; outR := out_map I |}).
+
+(* assumes: n ∈ domm I *)
+Definition inflow_delete_KT (I : KT_flowint_ur) (n: Node) 
+                            (k: K) (t: nat) :KT_flowint_ur := 
+           let I_inf_n := (nzmap_decrement (k,t) (inf I n)) in
+           let I'_inf := (<[ n := I_inf_n ]>(inf_map I)) in
+           (int {| infR := I'_inf ; outR := out_map I |}).
+
+Lemma inflow_insert_inset_ne_KT I n k t I' n' :
+      n' ≠ n → I' = inflow_insert_KT I n k t → 
+                inset_KT I' n' = inset_KT I n'.
+Proof.
+  intros Hneq Heq. unfold inset_KT.
+  unfold inf at 1. replace I'. 
+  unfold inflow_insert_KT. simpl.
+  rewrite lookup_insert_ne; try done.
+Qed.
+
+Lemma inflow_insert_inset_KT I n k t I' :
+      I' = inflow_insert_KT I n k t → 
+            inset_KT I' n = (inset_KT I n) ∪ {[(k,t)]}.
+Proof.
+  intros Heq. unfold inset_KT.
+  unfold inf at 1. replace I'. 
+  unfold inflow_insert_KT. simpl.
+  rewrite lookup_insert. 
+  apply leibniz_equiv. simpl.
+  destruct (decide (inf I n ! (k, t) + 1 = 0)); try lia.
+  rewrite nzmap_dom_insert_nonzero; try done.
+  set_solver.
+Qed.
+
+Lemma inflow_delete_inset_ne_KT I n k t I' n' :
+      n' ≠ n → I' = inflow_delete_KT I n k t → 
+            inset_KT I' n' = inset_KT I n'.
+Proof.
+  intros Hneq Heq. unfold inset_KT.
+  unfold inf at 1. replace I'. 
+  unfold inflow_delete_KT. simpl. 
+  rewrite lookup_insert_ne; try done.
+Qed.
+
+Lemma inflow_delete_inset_KT I n k t I' :
+      I' = inflow_delete_KT I n k t → 
+          ((inf I n ! (k,t) ≤ 1 → inset_KT I' n = (inset_KT I n) ∖ {[(k,t)]})
+          ∧ (inf I n ! (k,t) > 1 → inset_KT I' n = inset_KT I n)).
+Proof.
+  intros Heq. unfold inset_KT.
+  replace I'. split.
+  - intros le_1. unfold inflow_delete_KT.
+    unfold inf, inf_map at 1. simpl.
+    rewrite lookup_insert. simpl.
+    unfold nzmap_decrement.
+    destruct (inf_map I !! n) as [i | ] eqn:Hinf.
+    + simpl. destruct i as [ig prf_ig].
+      unfold dom, nzmap_dom. simpl.
+      unfold gmap_decrement.
+      rewrite /(inf I n ! (k, t)) in le_1.
+      unfold finmap_lookup_total in le_1.
+      unfold ccmunit, ccm_unit in le_1. 
+      simpl in le_1. unfold nat_unit in le_1.
+      unfold inf in le_1.
+      rewrite Hinf in le_1.
+      simpl in le_1.
+      assert (1 <? ig !!! (k,t) = false) as H'.
+      { apply PeanoNat.Nat.ltb_ge. 
+        rewrite /(ig !!! (k,t)).
+        unfold finmap_lookup_total.
+        unfold inhabitant. by simpl. }
+      rewrite H'. apply leibniz_equiv.
+      by rewrite dom_delete.
+    + simpl. unfold gmap_decrement.
+      unfold nzmap_dom. simpl.
+      assert (1 <? (∅: gmap KT nat) !!! (k, t) = false) as H'.
+      { apply PeanoNat.Nat.ltb_ge.
+        rewrite /(∅ !!! (k, t)). 
+        unfold finmap_lookup_total. 
+        unfold inhabitant. simpl.
+        rewrite lookup_empty. simpl. lia. }
+      rewrite H'. apply leibniz_equiv.
+      by rewrite dom_delete.
+  - intros ge_1. unfold inflow_delete_KT.
+    unfold inf at 1, inf_map at 1. simpl.
+    rewrite lookup_insert. simpl.
+    unfold nzmap_decrement. 
+    destruct (inf I n) as [i prf_i] eqn: Hi.
+    unfold dom, nzmap_dom. simpl.
+    unfold gmap_decrement. 
+    rewrite <-Hi in ge_1. 
+    assert (1 <? i !!! (k,t) = true) as H'. 
+    { apply PeanoNat.Nat.ltb_lt.
+      unfold nzmap_total_lookup in ge_1.
+      rewrite /(inf I n !! (k, t)) in ge_1.
+      unfold nzmap_lookup in ge_1.
+      rewrite Hi in ge_1.
+      rewrite /(i !!! (k, t)).
+      unfold finmap_lookup_total.
+      unfold inhabitant. by simpl. }
+    rewrite H'. apply leibniz_equiv.
+    rewrite dom_insert.
+    assert ((k,t) ∈ dom (gset KT) i).
+    { rewrite elem_of_dom.
+      unfold nzmap_total_lookup in ge_1.
+      rewrite /(inf I n !! (k, t)) in ge_1.
+      unfold nzmap_lookup in ge_1.
+      rewrite Hi in ge_1.
+      destruct (i !! (k,t)) eqn: H''.
+      exists n0; try done. rewrite H'' in ge_1.
+      unfold ccmunit, ccm_unit in ge_1. 
+      simpl in ge_1. unfold nat_unit in ge_1. lia. }
+    set_solver.         
+Qed.
+
+Lemma inflow_insert_domm I n k t I' : 
+      I' = inflow_insert_KT I n k t → domm I' = domm I ∪ {[n]}.
+Proof.
+  intros Heq. unfold domm, dom, flowint_dom.
+  apply leibniz_equiv. apply elem_of_equiv.
+  intros n'. rewrite elem_of_union.
+  rewrite !elem_of_dom.
+  replace I'. unfold inflow_insert_KT. simpl.
+  destruct (decide (n' = n)). 
+  - replace n'. rewrite lookup_insert.
+    split. intros H'. right. set_solver.
+    intros H'. unfold is_Some.
+    by exists <<[ (k, t) := inf I n ! (k, t) + 1 ]>> (inf I n).
+  - rewrite lookup_insert_ne; try done.
+    split. intros; left; try done.
+    intros [H' | H']; try done.
+    assert (n' = n) by set_solver.
+    contradiction.      
+Qed.
+
+Lemma inflow_delete_domm I n k t I' : 
+      I' = inflow_delete_KT I n k t → domm I' = domm I ∪ {[n]}.
+Proof.
+  intros Heq. unfold domm, dom, flowint_dom.
+  apply leibniz_equiv. apply elem_of_equiv.
+  intros n'. rewrite elem_of_union.
+  rewrite !elem_of_dom.
+  replace I'. unfold inflow_delete_KT. simpl.
+  destruct (decide (n' = n)). 
+  - replace n'. rewrite lookup_insert.
+    split. intros H'. right. set_solver.
+    intros H'. unfold is_Some.
+    by exists (nzmap_decrement (k, t) (inf I n)).
+  - rewrite lookup_insert_ne; try done.
+    split. intros; left; try done.
+    intros [H' | H']; try done.
+    assert (n' = n) by set_solver.
+    contradiction.
+Qed.
+
+Lemma flowint_delete_infComp_KT I1 I1' I2 I2' n k t :
+      n ∈ domm I2 → 
+        1 ≤ out I1 n ! (k,t)   →
+          out I1 n ! (k,t) ≤ inf I2 n ! (k,t)  → 
+            I1' = outflow_delete_KT I1 n k t →
+              I2' = inflow_delete_KT I2 n k t →
+                infComp I1 I2 = infComp I1' I2'.
+Proof.
+  intros n_in_I2 kt_outI1 I2_ge_I1 Hi1 Hi2. apply map_eq. intros n'.
+  unfold infComp. rewrite !gmap_imerge_prf.
+  unfold infComp_op.
+  destruct (decide (n' = n)).
+  - replace n'.
+    assert (inf_map I1 !! n = inf_map I1' !! n) as Hin_eq.
+    { replace I1'. unfold inf_map. by simpl. }
+    assert (out I2 n = out I2' n) as Hon_eq.
+    { replace I2'. unfold inflow_delete_KT.
+      unfold out, out_map. by simpl. }  
+    destruct (inf_map I1 !! n) as [i1 | ] eqn: Hi1n.
+    + rewrite Hon_eq.
+      destruct (inf_map I1' !! n); by inversion Hin_eq.
+    + destruct (inf_map I1' !! n); inversion Hin_eq.
+      destruct (inf_map I2 !! n) as [i2 | ] eqn: Hi2n.
+      * replace I2'. simpl. rewrite lookup_insert.
+        unfold inf. rewrite Hi2n. simpl.
+        replace I1'. unfold outflow_delete_KT. 
+        unfold out, out_map at 2. simpl.
+        rewrite nzmap_lookup_total_insert.
+        apply f_equal. unfold ccmop_inv, ccm_opinv.
+        simpl. unfold lift_opinv. unfold ccmop_inv, ccm_opinv.
+        simpl. unfold nat_opinv.
+        apply nzmap_eq. intros [k' t'].
+        rewrite !nzmap_lookup_merge.
+        destruct (decide ((k,t) = (k', t'))).
+        ** inversion e0. replace k'. replace t'.
+           rewrite !nzmap_lookup_total_decrement.
+           assert (∀ (x y: nat), 1 ≤ x → 1 ≤ y → y ≤ x 
+                            → x - y = x - 1 - (y - 1)) as Heq. lia.
+           assert (1 ≤ (out_map I1 ! n) ! (k,t)). 
+           { by unfold out in kt_outI1. }
+           assert (1 ≤ i2 ! (k,t)). 
+           { unfold inf in I2_ge_I1. rewrite Hi2n in I2_ge_I1. 
+             simpl in I2_ge_I1. lia. }
+           apply Heq; try done.
+           unfold inf in I2_ge_I1. rewrite Hi2n in I2_ge_I1. 
+           by simpl in I2_ge_I1.
+        ** rewrite !nzmap_lookup_total_decrement_ne; try done.
+      * unfold domm, dom, flowint_dom in n_in_I2.
+        rewrite elem_of_dom in n_in_I2 *; intros n_in_I2.
+        rewrite Hi2n in n_in_I2. exfalso. 
+        destruct n_in_I2 as [x n_in_I2]. 
+        inversion n_in_I2. 
+  - assert (inf_map I1 !! n' = inf_map I1' !! n') as Eq1.
+    { replace I1'. unfold outflow_delete_KT.
+      unfold inf_map at 2. by simpl. }
+    assert (out I2 n' = out I2' n') as Eq2.
+    { replace I2'. unfold inflow_delete_KT. 
+      unfold out, out_map at 2. by simpl. }
+    assert (inf_map I2 !! n' = inf_map I2' !! n') as Eq3. 
+    { replace I2'. unfold inflow_delete_KT.
+      unfold inf_map at 2. simpl.
+      rewrite lookup_insert_ne; try done. }
+    assert (out I1 n' = out I1' n') as Eq4.
+    { replace I1'. unfold outflow_delete_KT.
+      unfold out, out_map at 2. simpl.
+      rewrite nzmap_lookup_total_insert_ne; try done. }
+    by rewrite Eq1 Eq2 Eq3 Eq4.       
+Qed.
+
+Lemma flowint_delete_outComp_KT I1 I1' I2 I2' n k t :
+      n ∈ domm I2 → 
+        I1' = outflow_delete_KT I1 n k t →
+          I2' = inflow_delete_KT I2 n k t →
+            outComp I1 I2 = outComp I1' I2'.
+Proof.
+  intros n_in_I2 Hi1 Hi2. apply nzmap_eq. intros n'.
+  unfold outComp. rewrite !nzmap_lookup_imerge.
+  unfold outComp_op.
+  pose proof (inflow_delete_domm I2 n k t I2' Hi2) as domm_2.
+  destruct (decide (n' = n)).
+  - replace n'.
+    assert (n ∈ domm I2') as n_in_I2' by set_solver.
+    destruct (decide (n ∈ domm I1 ∪ domm I2)); 
+    last by set_solver.
+    by destruct (decide (n ∈ domm I1' ∪ domm I2')); 
+    last by set_solver.
+  - destruct (decide (n' ∈ domm I1 ∪ domm I2)).
+    + assert (n' ∈ domm I1' ∪ domm I2') as n'_in_I12' by set_solver.
+      by destruct (decide (n' ∈ domm I1' ∪ domm I2')); last by set_solver.
+    + assert (n' ∉ domm I1' ∪ domm I2') as n_notin_I12' by set_solver.
+      destruct (decide (n' ∈ domm I1' ∪ domm I2')); first by set_solver.
+      unfold ccmop, ccm_op. simpl. unfold lift_op, ccmop, ccm_op.
+      simpl. apply nzmap_eq. intros kt'.
+      rewrite !nzmap_lookup_merge. unfold nat_op.
+      replace I1'. unfold outflow_delete_KT. unfold out_map at 3.
+      simpl. rewrite nzmap_lookup_total_insert_ne; try done.
+      replace I2'. unfold inflow_delete_KT. unfold out_map at 4.
+      by simpl. 
+Qed.
+
+Lemma outflow_delete_valid_KT I1 I1' n k t :
+      I1' = outflow_delete_KT I1 n k t →
+          ✓ I1 → ✓ I1'.
+Proof.
+  intros Hi1_eq Valid1.
+  unfold valid, flowint_valid.
+  replace I1'. unfold outflow_delete_KT.
+  simpl.
+  unfold nzmap_insert.
+  destruct (decide (nzmap_decrement (k, t) (out I1 n) = 0%CCM)).
+  - destruct (I1) as [ [i o] | ] eqn: Hi1; [| exfalso; try done].
+    simpl. unfold nzmap_delete.
+    destruct o as [og prf_og] eqn: Hog.
+    simpl. repeat split.
+    + unfold valid, flowint_valid in Valid1. 
+      simpl in Valid1. 
+      destruct Valid1 as [H' _].
+      rewrite map_disjoint_spec in H' *; intros H'.
+      rewrite map_disjoint_spec.
+      intros n' mi mo Hmi Hmo.
+      destruct (decide (n' = n)).
+      * subst n'. rewrite lookup_delete in Hmo.
+        inversion Hmo.
+      * rewrite lookup_delete_ne in Hmo; try done.
+        by pose proof H' n' mi mo Hmi Hmo.
+   + intros Hi0. apply nzmap_eq. intros n'.
+     unfold nzmap_total_lookup at 1, lookup at 1.
+     unfold nzmap_lookup.
+     destruct (decide (n' = n)).
+     * subst n'.
+       rewrite lookup_delete. simpl.
+       by rewrite nzmap_lookup_empty.
+     * rewrite lookup_delete_ne; try done.
+       unfold valid, flowint_valid in Valid1. 
+       simpl in Valid1. 
+       destruct Valid1 as [_ H'].
+       pose proof H' Hi0 as H'.
+       rewrite nzmap_eq in H' *; intros H'.
+       pose proof H' n' as H'.
+       by unfold nzmap_total_lookup at 1, lookup at 1,
+            nzmap_lookup at 1 in H'.
+  - destruct (I1) as [ [i o] | ] eqn: Hi1; [| exfalso; try done].
+    simpl. unfold out, out_map. simpl.                
+    destruct o as [og prf_og] eqn: Hog.
+    simpl. split.
+    + unfold valid, flowint_valid in Valid1. 
+      simpl in Valid1. 
+      destruct Valid1 as [H' _].
+      rewrite map_disjoint_spec in H' *; intros H'.
+      rewrite map_disjoint_spec.
+      intros n' mi mo Hmi Hmo.
+      destruct (decide (n' = n)).
+      * subst n'. rewrite lookup_insert in Hmo.
+        inversion Hmo. rewrite <-Hog in H1.
+        clear Hmo. rename H1 into Hmo. 
+        unfold nzmap_decrement in Hmo.
+        destruct (o !! n) as [ogn | ] eqn: Hon.
+        ** rewrite Hog in Hon. 
+           unfold lookup, nzmap_lookup in Hon.
+           apply (H' n mi ogn); try done.
+        ** unfold out, out_map in n0. simpl in n0.    
+           rewrite <-Hog in n0. unfold nzmap_total_lookup in n0.
+           rewrite Hon in n0. simpl in n0.
+           unfold ccmunit, lift_unit in n0.
+           rewrite nzmap_empty_lookup in n0 *; intros n0.
+           destruct n0 as [kt' n0].
+           unfold ccmunit, ccm_unit in n0. simpl in n0.
+           unfold nat_unit in n0.
+           unfold nzmap_total_lookup in n0.
+           unfold lookup, nzmap_lookup in n0.
+           unfold gmap_decrement in n0.
+           assert ((∅: gmap KT nat) !!! (k,t) = 0) as H''.
+           { unfold lookup_total, finmap_lookup_total.
+             rewrite lookup_empty. by simpl. }
+           rewrite H'' in n0.
+           destruct (1 <? 0) eqn: Harith.
+           apply Nat.ltb_lt in Harith. lia.
+           destruct (decide (kt' = (k,t))). 
+           subst kt'. rewrite lookup_delete in n0. simpl in n0.
+           unfold ccmunit, nat_unit in n0. done. 
+           rewrite lookup_delete_ne in n0; try done. 
+      * rewrite lookup_insert_ne in Hmo; try done.
+        by pose proof H' n' mi mo Hmi Hmo.
+    + intros Hi0. apply nzmap_eq. intros n'.             
+      unfold valid, flowint_valid in Valid1.
+      destruct Valid1 as [_ H'].
+      simpl in H'. pose proof H' Hi0 as H'.
+      rewrite <-Hog in H'.
+      unfold nzmap_total_lookup at 1, lookup at 1.
+      unfold nzmap_lookup.
+      destruct (decide (n' = n)).
+      * subst n'. rewrite lookup_insert.
+        simpl. rewrite <-Hog.
+        rewrite nzmap_lookup_empty.
+        apply nzmap_eq. intros kt'.
+        rewrite H'.
+        unfold ccmunit, ccm_unit. simpl.
+        unfold lift_unit.
+        rewrite nzmap_lookup_empty.
+        unfold ccmunit, ccm_unit. simpl.
+        unfold nat_unit. unfold nzmap_total_lookup.
+        unfold lookup, nzmap_lookup.
+        unfold gmap_decrement.
+        assert ((∅: gmap KT nat) !!! (k,t) = 0) as H''.
+        { unfold lookup_total, finmap_lookup_total.
+          rewrite lookup_empty. by simpl. }
+        rewrite H''.
+        destruct (1 <? 0) eqn: Harith.
+        apply Nat.ltb_lt in Harith. lia.
+        destruct (decide (kt' = (k,t))). 
+        replace kt'. rewrite lookup_delete.
+        by simpl. rewrite lookup_delete_ne; try done.
+      * rewrite lookup_insert_ne; try done.
+        rewrite nzmap_eq in H' *; intros H'.
+        pose proof H' n' as H'.
+        unfold nzmap_total_lookup at 1 in H'.
+        rewrite Hog in H'. 
+        by unfold lookup at 1, nzmap_lookup at 1 in H'.
+Qed.
+
+Lemma inflow_delete_valid_KT I1 I1' n k t :
+      n ∈ domm I1 →
+        I1' = inflow_delete_KT I1 n k t →
+          ✓ I1 → ✓ I1'.
+Proof.
+  intros n_domm Hi1_eq Valid1.
+  unfold valid, flowint_valid.
+  replace I1'. unfold inflow_delete_KT. 
+  destruct (I1) as [ [i o] | ] eqn: Hi1; [| exfalso; try done].
+  unfold valid, flowint_valid in Valid1. 
+  simpl in Valid1. 
+  simpl. split.
+  - apply map_disjoint_dom.
+    simpl.
+    destruct Valid1 as [H' _].
+    apply map_disjoint_dom in H'. rewrite <-Hi1 in Hi1_eq.
+    pose proof (inflow_delete_domm I1 n k t I1' Hi1_eq) as Hdomm.
+    rewrite <-Hi1 in n_domm.
+    assert (domm I1' = domm I1) as H'' by set_solver.
+    unfold domm, dom, flowint_dom in H''.
+    replace I1' in H''. unfold inflow_delete_KT in H''.
+    simpl in H''. rewrite Hi1 in H''. simpl in H''.
+    rewrite <-Hi1 in H''. apply leibniz_equiv_iff in H''.
+    rewrite (dom_insert i) in H'' *; intros H''.
+    unfold domm, dom, flowint_dom in n_domm.
+    replace I1 in n_domm. simpl in n_domm.
+    rewrite dom_insert. set_solver.
+  - intros Hi. destruct Valid1 as [_ H'].
+    apply nzmap_eq. intros n'.
+    rewrite <-Hi1 in Hi. 
+    assert (<[n:=nzmap_decrement (k, t) (inf I1 n)]> i !! n = None) as H''.
+    { rewrite Hi. by rewrite lookup_empty. }
+    rewrite lookup_insert in H''.
+    inversion H''.
+Qed.    
+
+Lemma flowint_delete_intComposable_KT I1 I1' I2 I2' n k t :
+      n ∈ domm I2 → 
+        out I1 n ! (k,t) ≤ inf I2 n ! (k,t) →
+          I1' = outflow_delete_KT I1 n k t →
+            I2' = inflow_delete_KT I2 n k t →
+              intComposable I1 I2 → 
+                intComposable I1' I2'.
+Proof.
+  intros n_in_I2 I2_ge_I1 Hi1 Hi2 Intcomp. unfold intComposable.
+  repeat split.
+  - apply (outflow_delete_valid_KT I1 I1' n k t); try done.
+    by destruct Intcomp as [H' _].
+  - apply (inflow_delete_valid_KT I2 I2' n k t); try done.
+    by destruct Intcomp as [_ [H' _]].
+  - pose proof (inflow_delete_domm I2 n k t I2' Hi2) as domm_2.
+    assert (domm I1' = domm I1) as domm_1. 
+    { unfold domm, dom, flowint_dom. replace I1'.
+      unfold outflow_delete_KT. unfold inf_map. by simpl. }
+    destruct Intcomp as [_ [_ [H' _]]].
+    set_solver.
+  - unfold map_Forall.
+    intros n' m. intros Hin'. apply nzmap_eq. intros kt'.
+    unfold ccmop, ccm_op. simpl. unfold lift_op, ccmop, ccm_op.
+    simpl. unfold ccmop_inv, ccm_opinv.
+    simpl. unfold lift_opinv. unfold ccmop_inv, ccm_opinv. simpl.
+    rewrite !nzmap_lookup_merge. unfold nat_op, nat_opinv.
+    assert (inf_map I1' = inf_map I1) as Hinf_1.
+    { replace I1'. unfold outflow_delete_KT.
+      unfold inf_map. by simpl. }
+    rewrite Hinf_1 in Hin'.
+    destruct Intcomp as [_ [_ [_ [H' _]]]].
+    unfold map_Forall in H'. pose proof H' n' m Hin' as H'.  
+    unfold ccmop, ccm_op in H'. simpl in H'. unfold lift_op, ccmop, ccm_op in H'.
+    simpl in H'. unfold ccmop_inv, ccm_opinv in H'.
+    simpl in H'. unfold lift_opinv in H'. unfold ccmop_inv, ccm_opinv in H'.
+    simpl in H'. rewrite nzmap_eq in H' *; intros H'.
+    pose proof H' kt' as H'. rewrite !nzmap_lookup_merge in H'.
+    unfold nat_op, nat_opinv in H'.
+    assert (out I2' n' = out I2 n') as Hout.
+    { replace I2'. unfold inflow_delete_KT.
+      unfold out, out_map. by simpl. }
+    rewrite Hout. unfold inf. unfold inf in H'.
+    by rewrite Hinf_1.
+  - unfold map_Forall.
+    intros n' m. intros Hin'. apply nzmap_eq. intros kt'.
+    unfold ccmop, ccm_op. simpl. unfold lift_op, ccmop, ccm_op.
+    simpl. unfold ccmop_inv, ccm_opinv.
+    simpl. unfold lift_opinv. unfold ccmop_inv, ccm_opinv. simpl.
+    rewrite !nzmap_lookup_merge. unfold nat_op, nat_opinv.
+    destruct Intcomp as [_ [_ [_ [_ H']]]].
+    unfold map_Forall in H'. pose proof H' n' as H'.  
+    unfold ccmop, ccm_op in H'. simpl in H'. unfold lift_op, ccmop, ccm_op in H'.
+    simpl in H'. unfold ccmop_inv, ccm_opinv in H'.
+    simpl in H'. unfold lift_opinv in H'. unfold ccmop_inv, ccm_opinv in H'.
+    simpl in H'. destruct (decide (n' = n)). 
+    + replace n'. replace I1'. unfold outflow_delete_KT.
+      unfold out at 1, out_map at 1. simpl.
+      unfold out at 2, out_map at 2. simpl.
+      rewrite !nzmap_lookup_total_insert.
+      destruct (decide (kt' = (k,t))).
+      * replace kt'. rewrite nzmap_lookup_total_decrement.
+        replace I2' in Hin'. unfold inflow_delete_KT in Hin'.
+        unfold inf_map at 1 in Hin'. simpl in Hin'.
+        rewrite e in Hin'. rewrite lookup_insert in Hin'.
+        inversion Hin'. rewrite nzmap_lookup_total_decrement.
+        replace I2'. unfold inflow_delete_KT.
+        unfold inf at 2. unfold inf_map at 1. simpl.
+        rewrite lookup_insert. simpl.
+        rewrite nzmap_lookup_total_decrement.
+        assert (∀ (x y: nat), x >= y →
+            x - 1 = y - 1 + (x - 1 - (y - 1))) as Heq. lia.
+        apply Heq; try done.
+      * unfold inf. rewrite e in Hin'. rewrite Hin'. simpl.
+        replace I2' in Hin'. unfold inflow_delete_KT in Hin'. 
+        unfold inf_map at 1 in Hin'. simpl in Hin'. 
+        rewrite lookup_insert in Hin'. inversion Hin'.
+        rename H1 into Hin2.
+        rewrite !nzmap_lookup_total_decrement_ne; try done.
+        rewrite e in H'.
+        assert (inf_map I2 !! n = Some (inf I2 n)) as H''.
+        { unfold inf. destruct (inf_map I2 !! n) eqn: Hi2n.
+          by simpl. unfold domm, dom, flowint_dom in n_in_I2.
+          rewrite elem_of_dom in n_in_I2 *; intros n_in_I2.
+          rewrite Hi2n in n_in_I2. 
+          destruct n_in_I2 as [x Hx]; inversion Hx. } 
+        pose proof H' (inf I2 n) H'' as Heq.
+        rewrite nzmap_eq in Heq *; intros Heq.
+        pose proof Heq kt' as Heq. 
+        rewrite !nzmap_lookup_merge in Heq.
+        by unfold nat_op, nat_opinv in Heq.
+    + assert (inf I2' n' = inf I2 n') as Hin. 
+      { replace I2'. unfold inflow_delete_KT.
+      unfold inf at 1, inf_map at 1. simpl.
+      rewrite lookup_insert_ne; try done. }
+      rewrite Hin. replace I2' in Hin'. 
+      unfold inflow_delete_KT in Hin'.
+      unfold inf at 1, inf_map at 1 in Hin'. simpl in Hin'.
+      rewrite lookup_insert_ne in Hin'; try done. 
+      pose proof H' m Hin' as H'.
+      rewrite nzmap_eq in H' *; intros H'.
+      pose proof H' kt' as H'.
+      rewrite !nzmap_lookup_merge in H'.
+      unfold nat_op, nat_opinv in H'.
+      assert (out I1' n' = out I1 n') as Hout.
+      { replace I1'. unfold outflow_delete_KT.
+        unfold out at 1, out_map at 1. simpl.
+        rewrite nzmap_lookup_total_insert_ne; try done. }
+      by rewrite Hout.  
+Qed.
+
+Lemma flowint_delete_valid_KT I1 I1' I2 I2' n k t :
+        n ∈ domm I2 →
+          I1' = outflow_delete_KT I1 n k t →
+            I2' = inflow_delete_KT I2 n k t →
+              ✓ (I1 ⋅ I2) → ✓ (I1' ⋅ I2').
+Proof.
+  intros n_in_I2 Hi1 Hi2 Valid_12.
+  pose proof intComposable_valid I1 I2 Valid_12 as Intcomp_12.
+  apply intValid_composable. 
+  apply (flowint_delete_intComposable_KT I1 I1' I2 I2' n k t); try done.
+  pose proof intComp_unfold_inf_2 I1 I2 Valid_12 n n_in_I2 as H'.
+  unfold ccmop, ccm_op in H'. simpl in H'.
+  unfold lift_op, ccmop, ccm_op in H'. simpl in H'.
+  rewrite nzmap_eq in H' *; intros H'.
+  pose proof H' (k,t) as H'. unfold nat_op in H'.
+  rewrite nzmap_lookup_merge in H'. 
+  rewrite H'.
+  assert (∀ (x y: nat), x ≤ y + x) as Heq by lia.
+  apply Heq.
+Qed.
+
+
+Lemma flowint_delete_eq_KT I1 I1' I2 I2' n k t :
+      n ∈ domm I2 → 
+        1 ≤ out I1 n ! (k, t) →
+          I1' = outflow_delete_KT I1 n k t →
+            I2' = inflow_delete_KT I2 n k t →
+              ✓ (I1 ⋅ I2) → I1 ⋅ I2 = I1' ⋅ I2'.
+Proof.
+  intros n_in_I2 Hout1 Hi1 Hi2 Valid_12.
+  pose proof (intComposable_valid _ _ Valid_12) as HintComp.
+  pose proof (flowint_delete_valid_KT I1 I1' I2 I2' n k t 
+                      n_in_I2 Hi1 Hi2 Valid_12) as Valid_12'.
+  pose proof (intComposable_valid _ _ Valid_12') as HintComp'.   
+  destruct (I1⋅I2) as [ [i o] | ] eqn: Hi12; [| exfalso; try done].
+  unfold op, intComp in Hi12.
+  destruct (decide (intComposable I1 I2)); last done.
+  inversion Hi12.
+  destruct (I1'⋅I2') as [ [i' o'] | ] eqn: Hi12'; [| exfalso; try done].    
+  unfold op, intComp in Hi12'.
+  destruct (decide (intComposable I1' I2')); last done.
+  inversion Hi12'.
+  apply intValid_composable in HintComp.
+  assert (infComp I1 I2 = infComp I1' I2') as Hinfcomp.
+  { apply (flowint_delete_infComp_KT I1 I1' I2 I2' n k t); try done.
+    pose proof intComp_unfold_inf_2 I1 I2 HintComp n n_in_I2 as H'.
+    unfold ccmop, ccm_op in H'. simpl in H'.
+    unfold lift_op, ccmop, ccm_op in H'. simpl in H'.
+    rewrite nzmap_eq in H' *; intros H'.
+    pose proof H' (k,t) as H'. unfold nat_op in H'.
+    rewrite nzmap_lookup_merge in H'. 
+    rewrite H'.
+    assert (∀ (x y: nat), x ≤ y + x) as Heq by lia.
+    apply Heq. }
+  pose proof (flowint_delete_outComp_KT I1 I1' I2 I2' n k t n_in_I2 Hi1 Hi2) 
+                                      as Houtcomp.
+  by rewrite Hinfcomp Houtcomp.
+Qed.
+
+Lemma flowint_insert_infComp_KT I1 I1' I2 I2' n k t :
+      n ∈ domm I2 → 
+          out I1 n ! (k,t) ≤ inf I2 n ! (k,t)  → 
+            I1' = outflow_insert_KT I1 n k t →
+              I2' = inflow_insert_KT I2 n k t →
+                infComp I1 I2 = infComp I1' I2'.
+Proof.
+  intros n_in_I2 I2_ge_I1 Hi1 Hi2. apply map_eq.
+  intros n'. unfold infComp. rewrite !gmap_imerge_prf.
+  unfold infComp_op.
+  destruct (decide (n' = n)).
+  - replace n'.
+    assert (inf_map I1 !! n = inf_map I1' !! n) as Hin_eq.
+    { replace I1'. unfold inf_map. by simpl. }
+    assert (out I2 n = out I2' n) as Hon_eq.
+    { replace I2'. unfold inflow_delete_KT.
+      unfold out, out_map. by simpl. }  
+    destruct (inf_map I1 !! n) as [i1 | ] eqn: Hi1n.
+    + rewrite Hon_eq.
+      destruct (inf_map I1' !! n); by inversion Hin_eq.
+    + destruct (inf_map I1' !! n); inversion Hin_eq.
+      destruct (inf_map I2 !! n) as [i2 | ] eqn: Hi2n.
+      * replace I2'. simpl. rewrite lookup_insert.
+        apply f_equal.
+        unfold inf. rewrite Hi2n. simpl.
+        replace I1'. unfold outflow_insert_KT. 
+        unfold out, out_map at 2. simpl.
+        rewrite nzmap_lookup_total_insert.
+        unfold ccmop_inv, ccm_opinv.
+        simpl. unfold lift_opinv. unfold ccmop_inv, ccm_opinv.
+        simpl. unfold nat_opinv.
+        apply nzmap_eq. intros [k' t'].
+        rewrite !nzmap_lookup_merge.
+        destruct (decide ((k,t) = (k', t'))).
+        ** inversion e0. replace k'. replace t'.
+           rewrite !nzmap_lookup_total_insert.
+           assert (∀ (x y: nat), y ≤ x 
+                            → x - y = x + 1 - (y + 1)) as Heq. lia.
+           apply Heq; try done.
+           unfold inf in I2_ge_I1. rewrite Hi2n in I2_ge_I1. 
+           by simpl in I2_ge_I1.
+        ** rewrite !nzmap_lookup_total_insert_ne; try done.
+      * unfold domm, dom, flowint_dom in n_in_I2.
+        rewrite elem_of_dom in n_in_I2 *; intros n_in_I2.
+        rewrite Hi2n in n_in_I2. exfalso. 
+        destruct n_in_I2 as [x n_in_I2]. 
+        inversion n_in_I2. 
+  - assert (inf_map I1 !! n' = inf_map I1' !! n') as Eq1.
+    { replace I1'. unfold outflow_delete_KT.
+      unfold inf_map at 2. by simpl. }
+    assert (out I2 n' = out I2' n') as Eq2.
+    { replace I2'. unfold inflow_delete_KT. 
+      unfold out, out_map at 2. by simpl. }
+    assert (inf_map I2 !! n' = inf_map I2' !! n') as Eq3. 
+    { replace I2'. unfold inflow_delete_KT.
+      unfold inf_map at 2. simpl.
+      rewrite lookup_insert_ne; try done. }
+    assert (out I1 n' = out I1' n') as Eq4.
+    { replace I1'. unfold outflow_delete_KT.
+      unfold out, out_map at 2. simpl.
+      rewrite nzmap_lookup_total_insert_ne; try done. }
+    by rewrite Eq1 Eq2 Eq3 Eq4.
+Qed.           
+    
+Lemma flowint_insert_outComp_KT I1 I1' I2 I2' n k t :
+      n ∈ domm I2 → 
+        I1' = outflow_insert_KT I1 n k t →
+          I2' = inflow_insert_KT I2 n k t →
+            outComp I1 I2 = outComp I1' I2'.
+Proof.
+  intros n_in_I2 Hi1 Hi2. apply nzmap_eq. intros n'.
+  unfold outComp. rewrite !nzmap_lookup_imerge.
+  unfold outComp_op.
+  pose proof (inflow_insert_domm I2 n k t I2' Hi2) as domm_2.
+  destruct (decide (n' = n)).
+  - replace n'.
+    assert (n ∈ domm I2') as n_in_I2' by set_solver.
+    destruct (decide (n ∈ domm I1 ∪ domm I2)); 
+    last by set_solver.
+    by destruct (decide (n ∈ domm I1' ∪ domm I2')); 
+    last by set_solver.
+  - destruct (decide (n' ∈ domm I1 ∪ domm I2)).
+    + assert (n' ∈ domm I1' ∪ domm I2') as n'_in_I12' by set_solver.
+      by destruct (decide (n' ∈ domm I1' ∪ domm I2')); last by set_solver.
+    + assert (n' ∉ domm I1' ∪ domm I2') as n_notin_I12' by set_solver.
+      destruct (decide (n' ∈ domm I1' ∪ domm I2')); first by set_solver.
+      unfold ccmop, ccm_op. simpl. unfold lift_op, ccmop, ccm_op.
+      simpl. apply nzmap_eq. intros kt'.
+      rewrite !nzmap_lookup_merge. unfold nat_op.
+      replace I1'. unfold outflow_delete_KT. unfold out_map at 3.
+      simpl. rewrite nzmap_lookup_total_insert_ne; try done.
+      replace I2'. unfold inflow_delete_KT. unfold out_map at 4.
+      by simpl. 
+Qed.
+
+Lemma outflow_insert_valid_KT I1 I1' n k t :
+      n ∉ domm I1 → 
+        domm I1 ≠ ∅ →
+          I1' = outflow_insert_KT I1 n k t →
+            ✓ I1 → ✓ I1'.
+Proof.
+  intros n_domm domm_I1 Hi1_eq Valid1.
+  unfold valid, flowint_valid.
+  replace I1'. unfold inflow_insert_KT. 
+  destruct (I1) as [ [i o] | ] eqn: Hi1; [| exfalso; try done].
+  unfold valid, flowint_valid in Valid1. 
+  simpl in Valid1. 
+  simpl. split.
+  - apply map_disjoint_dom.
+    destruct Valid1 as [H' _].
+    apply map_disjoint_dom in H'.
+    rewrite <-Hi1.
+    unfold nzmap_insert at 1.
+    destruct (decide (<<[ (k, t) := out I1 n ! (k, t) + 1 ]>> (out I1 n) = 0%CCM)).
+    + simpl. destruct o as [og prf_og] eqn: Ho.
+      unfold nzmap_delete. simpl. rewrite dom_delete.
+      set_solver.
+    + simpl. destruct o as [og prf_og] eqn: Ho.
+      simpl. rewrite dom_insert.
+      unfold domm, dom, flowint_dom in n_domm.
+      unfold inf_map in n_domm. simpl in n_domm.
+      set_solver. 
+  - intros Hi. destruct Valid1 as [_ H'].
+    unfold domm, dom, flowint_dom in domm_I1.
+    unfold inf_map in domm_I1. simpl in domm_I1.
+    exfalso. apply domm_I1. rewrite Hi. 
+    apply leibniz_equiv. by rewrite dom_empty.
+Qed.
+
+Lemma inflow_insert_valid_KT I1 I1' n k t :
+      n ∈ domm I1 →
+        I1' = inflow_insert_KT I1 n k t →
+          ✓ I1 → ✓ I1'.
+Proof.
+  intros n_domm Hi1_eq Valid1.
+  unfold valid, flowint_valid.
+  replace I1'. unfold inflow_insert_KT. 
+  destruct (I1) as [ [i o] | ] eqn: Hi1; [| exfalso; try done].
+  unfold valid, flowint_valid in Valid1. 
+  simpl in Valid1. 
+  simpl. split.
+  - apply map_disjoint_dom.
+    simpl.
+    destruct Valid1 as [H' _].
+    apply map_disjoint_dom in H'. rewrite <-Hi1 in Hi1_eq.
+    pose proof (inflow_insert_domm I1 n k t I1' Hi1_eq) as Hdomm.
+    rewrite <-Hi1 in n_domm.
+    assert (domm I1' = domm I1) as H'' by set_solver.
+    unfold domm, dom, flowint_dom in H''.
+    replace I1' in H''. unfold inflow_insert_KT in H''.
+    simpl in H''. rewrite Hi1 in H''. simpl in H''.
+    rewrite <-Hi1 in H''. apply leibniz_equiv_iff in H''.
+    rewrite (dom_insert i) in H'' *; intros H''.
+    unfold domm, dom, flowint_dom in n_domm.
+    replace I1 in n_domm. simpl in n_domm.
+    rewrite dom_insert. set_solver.
+  - intros Hi. destruct Valid1 as [_ H'].
+    apply nzmap_eq. intros n'.
+    rewrite <-Hi1 in Hi. 
+    assert (<[n:=<<[ (k, t) := inf I1 n ! (k, t) + 1 ]>> (inf I1 n)]> i !! n 
+                                  = None) as H''.
+    { rewrite Hi. by rewrite lookup_empty. }
+    rewrite lookup_insert in H''.
+    inversion H''.
+Qed.    
+
+Lemma flowint_insert_intComposable_KT I1 I1' I2 I2' n k t :
+       n ∈ domm I2 → domm I1 ≠ ∅ →
+        out I1 n ! (k,t) ≤ inf I2 n ! (k,t) →
+          I1' = outflow_insert_KT I1 n k t →
+            I2' = inflow_insert_KT I2 n k t →
+              intComposable I1 I2 → 
+                intComposable I1' I2'.
+Proof.
+  intros n_in_I2 domm_I1 I2_ge_I1 Hi1 Hi2 Intcomp.
+  assert (n ∉ domm I1) as n_notin_I1.
+  { unfold intComposable in Intcomp.
+    destruct Intcomp as [_ [_ [H' _]]].
+    clear -H' n_in_I2. set_solver. }
+  unfold intComposable. repeat split.
+  - apply (outflow_insert_valid_KT I1 I1' n k t); try done.
+    by destruct Intcomp as [H' _].
+  - apply (inflow_insert_valid_KT I2 I2' n k t); try done.
+    by destruct Intcomp as [_ [H' _]].
+  - pose proof (inflow_insert_domm I2 n k t I2' Hi2) as domm_2.
+    assert (domm I1' = domm I1) as domm_1. 
+    { unfold domm, dom, flowint_dom. replace I1'.
+      unfold outflow_insert_KT. unfold inf_map. by simpl. }
+    destruct Intcomp as [_ [_ [H' _]]].
+    set_solver.
+  - unfold map_Forall.
+    intros n' m. intros Hin'. apply nzmap_eq. intros kt'.
+    unfold ccmop, ccm_op. simpl. unfold lift_op, ccmop, ccm_op.
+    simpl. unfold ccmop_inv, ccm_opinv.
+    simpl. unfold lift_opinv. unfold ccmop_inv, ccm_opinv. simpl.
+    rewrite !nzmap_lookup_merge. unfold nat_op, nat_opinv.
+    assert (inf_map I1' = inf_map I1) as Hinf_1.
+    { replace I1'. unfold outflow_delete_KT.
+      unfold inf_map. by simpl. }
+    rewrite Hinf_1 in Hin'.
+    destruct Intcomp as [_ [_ [_ [H' _]]]].
+    unfold map_Forall in H'. pose proof H' n' m Hin' as H'.  
+    unfold ccmop, ccm_op in H'. simpl in H'. unfold lift_op, ccmop, ccm_op in H'.
+    simpl in H'. unfold ccmop_inv, ccm_opinv in H'.
+    simpl in H'. unfold lift_opinv in H'. unfold ccmop_inv, ccm_opinv in H'.
+    simpl in H'. rewrite nzmap_eq in H' *; intros H'.
+    pose proof H' kt' as H'. rewrite !nzmap_lookup_merge in H'.
+    unfold nat_op, nat_opinv in H'.
+    assert (out I2' n' = out I2 n') as Hout.
+    { replace I2'. unfold inflow_delete_KT.
+      unfold out, out_map. by simpl. }
+    rewrite Hout. unfold inf. unfold inf in H'.
+    by rewrite Hinf_1.
+  - unfold map_Forall.
+    intros n' m. intros Hin'. apply nzmap_eq. intros kt'.
+    unfold ccmop, ccm_op. simpl. unfold lift_op, ccmop, ccm_op.
+    simpl. unfold ccmop_inv, ccm_opinv.
+    simpl. unfold lift_opinv. unfold ccmop_inv, ccm_opinv. simpl.
+    rewrite !nzmap_lookup_merge. unfold nat_op, nat_opinv.
+    destruct Intcomp as [_ [_ [_ [_ H']]]].
+    unfold map_Forall in H'. pose proof H' n' as H'.  
+    unfold ccmop, ccm_op in H'. simpl in H'. unfold lift_op, ccmop, ccm_op in H'.
+    simpl in H'. unfold ccmop_inv, ccm_opinv in H'.
+    simpl in H'. unfold lift_opinv in H'. unfold ccmop_inv, ccm_opinv in H'.
+    simpl in H'. destruct (decide (n' = n)). 
+    + replace n'. replace I1'. unfold outflow_insert_KT.
+      unfold out at 1, out_map at 1. simpl.
+      unfold out at 3, out_map at 3. simpl.
+      rewrite !nzmap_lookup_total_insert.
+      destruct (decide (kt' = (k,t))).
+      * replace kt'. rewrite !nzmap_lookup_total_insert.
+        replace I2' in Hin'. unfold inflow_insert_KT in Hin'.
+        unfold inf_map at 1 in Hin'. simpl in Hin'.
+        rewrite e in Hin'. rewrite lookup_insert in Hin'.
+        inversion Hin'. rewrite nzmap_lookup_total_insert.
+        replace I2'. unfold inflow_insert_KT.
+        unfold inf at 2. unfold inf_map at 1. simpl.
+        rewrite lookup_insert. simpl.
+        rewrite nzmap_lookup_total_insert.
+        assert (∀ (x y: nat), x >= y →
+            x + 1 = y + 1 + (x + 1 - (y + 1))) as Heq. lia.
+        apply Heq; try done.
+      * unfold inf. rewrite e in Hin'. rewrite Hin'. simpl.
+        replace I2' in Hin'. unfold inflow_insert_KT in Hin'. 
+        unfold inf_map at 1 in Hin'. simpl in Hin'. 
+        rewrite lookup_insert in Hin'. inversion Hin'.
+        rename H1 into Hin2.
+        rewrite !nzmap_lookup_total_insert_ne; try done.
+        rewrite e in H'.
+        assert (inf_map I2 !! n = Some (inf I2 n)) as H''.
+        { unfold inf. destruct (inf_map I2 !! n) eqn: Hi2n.
+          by simpl. unfold domm, dom, flowint_dom in n_in_I2.
+          rewrite elem_of_dom in n_in_I2 *; intros n_in_I2.
+          rewrite Hi2n in n_in_I2. 
+          destruct n_in_I2 as [x Hx]; inversion Hx. } 
+        pose proof H' (inf I2 n) H'' as Heq.
+        rewrite nzmap_eq in Heq *; intros Heq.
+        pose proof Heq kt' as Heq. 
+        rewrite !nzmap_lookup_merge in Heq.
+        by unfold nat_op, nat_opinv in Heq.
+    + assert (inf I2' n' = inf I2 n') as Hin. 
+      { replace I2'. unfold inflow_insert_KT.
+      unfold inf at 1, inf_map at 1. simpl.
+      rewrite lookup_insert_ne; try done. }
+      rewrite Hin. replace I2' in Hin'. 
+      unfold inflow_insert_KT in Hin'.
+      unfold inf at 1, inf_map at 1 in Hin'. simpl in Hin'.
+      rewrite lookup_insert_ne in Hin'; try done. 
+      pose proof H' m Hin' as H'.
+      rewrite nzmap_eq in H' *; intros H'.
+      pose proof H' kt' as H'.
+      rewrite !nzmap_lookup_merge in H'.
+      unfold nat_op, nat_opinv in H'.
+      assert (out I1' n' = out I1 n') as Hout.
+      { replace I1'. unfold outflow_insert_KT.
+        unfold out at 1, out_map at 1. simpl.
+        rewrite nzmap_lookup_total_insert_ne; try done. }
+      by rewrite Hout.  
+Qed.
+
+Lemma flowint_insert_valid_KT I1 I1' I2 I2' n k t :
+      n ∈ domm I2 → domm I1 ≠ ∅ →
+        I1' = outflow_insert_KT I1 n k t →
+          I2' = inflow_insert_KT I2 n k t →
+            ✓ (I1 ⋅ I2) → ✓ (I1' ⋅ I2').
+Proof.
+  intros n_in_I2 domm_I1 Hi1 Hi2 Valid_12.
+  pose proof intComposable_valid I1 I2 Valid_12 as Intcomp_12.
+  apply intValid_composable. 
+  apply (flowint_insert_intComposable_KT I1 I1' I2 I2' n k t); try done.
+  pose proof intComp_unfold_inf_2 I1 I2 Valid_12 n n_in_I2 as H'.
+  unfold ccmop, ccm_op in H'. simpl in H'.
+  unfold lift_op, ccmop, ccm_op in H'. simpl in H'.
+  rewrite nzmap_eq in H' *; intros H'.
+  pose proof H' (k,t) as H'. unfold nat_op in H'.
+  rewrite nzmap_lookup_merge in H'. 
+  rewrite H'.
+  assert (∀ (x y: nat), x ≤ y + x) as Heq by lia.
+  apply Heq.  
+Qed.
+
+Lemma flowint_insert_eq_KT I1 I1' I2 I2' n k t :
+      n ∈ domm I2 → domm I1 ≠ ∅ →
+        I1' = outflow_insert_KT I1 n k t →
+          I2' = inflow_insert_KT I2 n k t →
+            ✓ (I1 ⋅ I2) → I1 ⋅ I2 = I1' ⋅ I2'.
+Proof.
+  intros n_in_I2 domm_I1 Hi1 Hi2 Valid_12.
+  pose proof (intComposable_valid _ _ Valid_12) as HintComp.
+  pose proof (flowint_insert_valid_KT I1 I1' I2 I2' n k t 
+                n_in_I2 domm_I1 Hi1 Hi2 Valid_12) as Valid_12'.
+  pose proof (intComposable_valid _ _ Valid_12') as HintComp'.   
+  destruct (I1⋅I2) as [ [i o] | ] eqn: Hi12; [| exfalso; try done].
+  unfold op, intComp in Hi12.
+  destruct (decide (intComposable I1 I2)); last done.
+  inversion Hi12.
+  destruct (I1'⋅I2') as [ [i' o'] | ] eqn: Hi12'; [| exfalso; try done].    
+  unfold op, intComp in Hi12'.
+  destruct (decide (intComposable I1' I2')); last done.
+  inversion Hi12'.
+  apply intValid_composable in HintComp.
+  assert (infComp I1 I2 = infComp I1' I2') as Hinfcomp.
+  { apply (flowint_insert_infComp_KT I1 I1' I2 I2' n k t); try done.
+    pose proof intComp_unfold_inf_2 I1 I2 HintComp n n_in_I2 as H'.
+    unfold ccmop, ccm_op in H'. simpl in H'.
+    unfold lift_op, ccmop, ccm_op in H'. simpl in H'.
+    rewrite nzmap_eq in H' *; intros H'.
+    pose proof H' (k,t) as H'. unfold nat_op in H'.
+    rewrite nzmap_lookup_merge in H'. 
+    rewrite H'.
+    assert (∀ (x y: nat), x ≤ y + x) as Heq by lia.
+    apply Heq. }
+  pose proof (flowint_insert_outComp_KT I1 I1' I2 I2' n k t n_in_I2 Hi1 Hi2) 
+                                      as Houtcomp.
+  by rewrite Hinfcomp Houtcomp.  
+Qed.
+
+Lemma outflow_insert_inf_eq_KT I n k t I' :
+      I' = outflow_insert_KT I n k t → 
+        ∀ n', inset_KT I' n' = inset_KT I n'.
+Proof.
+  intros Heq. intros n'. unfold inset_KT. 
+  unfold inf. replace I'.
+  unfold outflow_insert_KT. by simpl. 
+Qed.
+
+Lemma outflow_delete_inf_eq_KT I n k t I' :
+      I' = outflow_delete_KT I n k t → 
+        ∀ n', inset_KT I' n' = inset_KT I n'.
+Proof.
+  intros Heq. intros n'. unfold inset_KT. 
+  unfold inf. replace I'.
+  unfold outflow_insert_KT. by simpl. 
+Qed.
+
+
 End KT_flows.
 
+Arguments KT _ : assert.
 Arguments KT_multiset _ {_ _} : assert.
 Arguments KT_flowint_ur _ {_ _} : assert.
  
